cp

low-level/Veritas.HashSet.fst
@@ -19,10 +19,13 @@ let flush_interleaving = ()
 
 open LowStar.BufferOps
 
+let hash_value_t = Hacl.Blake2b_32.lbytes 32
+let hash_value_buf = B.lbuffer u8 32
+
 // Relying on a somewhat recent kremlin optimization that removes pointers to unit
 noeq
 type state_s = {
-  acc: acc:B.buffer u8 { B.length acc == 32 };
+  acc: hash_value_buf;
   seen: B.pointer (G.erased (list hashable_bytes));
   key: key:B.buffer u8 { B.length key == 64 };
   g_key: G.erased t_key;
@@ -42,7 +45,8 @@ let key s =
 let footprint_s s =
   B.(loc_addr_of_buffer s.acc `loc_union` loc_addr_of_buffer s.seen `loc_union` loc_addr_of_buffer s.key)
 
-let invariant_s h s =
+unfold
+let invariant_s' h s =
   B.live h s.acc /\ B.freeable s.acc /\
   B.live h s.seen /\ B.freeable s.seen /\
   B.live h s.key /\ B.freeable s.key /\
@@ -50,7 +54,10 @@ let invariant_s h s =
   B.disjoint s.acc s.key /\
   B.disjoint s.seen s.key /\
   B.as_seq h s.acc == gfold_right (fold_and_hash s.g_key) (G.reveal (B.deref h s.seen)) zero /\
-  G.reveal s.g_key == B.as_seq h s.key
+  G.reveal s.g_key == B.as_seq h s.key /\
+  B.as_seq h s.key `Seq.equal` Seq.create 64 0uy
+
+let invariant_s = invariant_s'
 
 let invariant_loc_in_footprint _ _ =
   allow_inversion state_s
@@ -62,34 +69,136 @@ let frame _ _ _ _ =
   allow_inversion state_s
 
 #push-options "--ifuel 1 --fuel 1 --z3rlimit 50"
-let create_in r k' =
-  let h0 = ST.get () in
+let create_in r =
   let b = B.malloc r 0uy 32ul in
   let p = B.malloc r (G.hide ([] #hashable_bytes)) 1ul in
   let k = B.malloc r 0uy 64ul in
-  B.blit k' 0ul k 0ul 64ul;
-  let h1 = ST.get () in
-  B.modifies_only_not_unused_in B.loc_none h0 h1;
+  let h0 = ST.get () in
   [@inline_let]
-  let s: state_s = { acc = b; seen = p; key = k; g_key = B.as_seq h0 k' } in
+  let s: state_s = { acc = b; seen = p; key = k; g_key = B.as_seq h0 k } in
   B.malloc r s 1ul
 #pop-options
 
-assume val xor_inplace (b1: B.buffer u8) (b2: B.buffer u8): Stack unit
-  (requires (fun h0 ->
-    B.live h0 b1 /\ B.live h0 b2 /\
-    B.length b1 == B.length b2))
-  (ensures (fun h0 _ h1 ->
-    B.(modifies (loc_buffer b1) h0 h1) /\
-    B.as_seq h1 b1 == xor_bytes (B.as_seq h0 b1) (B.as_seq h0 b2)))
 
-#push-options "--fuel 1 --z3rlimit 200"
+let hash_value (s:Seq.seq U8.t { Seq.length s <= blake2_max_input_length })
+  : hash_value_t
+  = Hacl.Blake2b_32.spec s 64 (Seq.create 64 0uy) 32
+
+let aggregate_hash_value (h0 h1: hash_value_t)
+  : hash_value_t
+  = xor_bytes h0 h1
+
+let as_hash_value (b:hash_value_buf) (h:HS.mem) =
+  B.as_seq h b
+
+let as_hash_value_pfx (b:hash_value_buf) (h:HS.mem) (n:nat { n <= 32 }) =
+  Seq.slice (as_hash_value b h) 0 n
+
+val aggregate_hash_value_buf (b1: hash_value_buf) (b2: hash_value_buf)
+  : Stack unit
+    (requires fun h0 ->
+      B.live h0 b1 /\
+      B.live h0 b2 /\
+      B.disjoint b1 b2)
+    (ensures fun h0 _ h1 ->
+      B.(modifies (loc_buffer b1) h0 h1) /\
+      as_hash_value b1 h1 == aggregate_hash_value (as_hash_value b1 h0)
+                                                  (as_hash_value b2 h0))
+let aggregate_hash_value_buf b1 b2 =
+  let h0 = ST.get () in
+  let inv h (i:nat) =
+      let s1 = B.as_seq h0 b1 in
+      let s2 = B.as_seq h0 b2 in
+      i <= 32 /\
+      B.live h b1 /\
+      B.live h b2 /\
+      Seq.slice (B.as_seq h b1) i 32 `Seq.equal` Seq.slice s1 i 32 /\
+      B.modifies (B.loc_buffer b1) h0 h /\
+      as_hash_value_pfx b1 h i `Seq.equal`
+      xor_bytes (Seq.slice s1 0 i) (Seq.slice s2 0 i)
+  in
+  let extend_inv (h:HS.mem) (i:nat) (h':HS.mem)
+    : Lemma
+      (requires
+        inv h i /\
+        i < 32 /\
+        B.as_seq h' b1 ==
+        Seq.upd (B.as_seq h b1)
+                i
+                (U8.logxor
+                  (B.get h b1 i)
+                  (B.get h b2 i)))
+      (ensures (
+        let s1 = B.as_seq h0 b1 in
+        let s2 = B.as_seq h0 b2 in
+        as_hash_value_pfx b1 h' (i + 1) `Seq.equal`
+        xor_bytes (Seq.slice s1 0 (i + 1))
+                  (Seq.slice s2 0 (i + 1)) /\
+        Seq.slice (B.as_seq h' b1) (i + 1) 32 `Seq.equal`
+        Seq.slice s1 (i + 1) 32))
+    = let s1 = B.as_seq h0 b1 in
+      let s2 = B.as_seq h0 b2 in
+      let s1_h =  B.as_seq h b1 in
+      let s1_h' = B.as_seq h' b1 in
+      assert (as_hash_value_pfx b1 h' (i + 1) `Seq.equal`
+              Seq.snoc (as_hash_value_pfx b1 h i)
+                       (Seq.index s1_h' i));
+      assert (xor_bytes (Seq.slice s1 0 (i + 1))
+                        (Seq.slice s2 0 (i + 1)) `Seq.equal`
+              Seq.snoc
+                 (xor_bytes (Seq.slice s1 0 i)
+                            (Seq.slice s2 0 i))
+                 (U8.logxor (Seq.index s1 i) (Seq.index s2 i)));
+      assert (Seq.index (B.as_seq h b2) i == Seq.index s2 i);
+      assert (Seq.slice (B.as_seq h b1) i 32 == Seq.slice s1 i 32);
+      Seq.lemma_index_slice s1 i 32 0;
+      assert (Seq.index (B.as_seq h b1) i == Seq.index s1 i);
+      assert ((Seq.index s1_h' i) ==
+                 (U8.logxor (Seq.index s1 i) (Seq.index s2 i)));
+      assert (Seq.slice s1 (i + 1) 32 `Seq.equal` Seq.tail (Seq.slice s1 i 32));
+      assert (Seq.slice (B.as_seq h' b1) (i + 1) 32 `Seq.equal`
+               Seq.tail (Seq.slice (B.as_seq h' b1) i 32));
+      assert (Seq.slice (B.as_seq h' b1) (i + 1) 32 `Seq.equal`
+              Seq.slice s1 (i + 1) 32)
+  in
+  [@@inline_let]
+  let body (i:U32.t { U32.v i < 32 })
+    : Stack unit
+      (fun h -> inv h (U32.v i))
+      (fun h0 _ h1 -> inv h1 (U32.v i + 1))
+    = let h = ST.get () in
+      let v1 = B.index b1 i in
+      let v2 = B.index b2 i in
+      B.upd b1 i (U8.logxor v1 v2);
+      let h' = ST.get () in
+      extend_inv h (U32.v i) h'
+  in
+  assert (inv h0 0);
+  let _ =
+    C.Loops.for 0ul 32ul inv body
+  in
+  let h = ST.get () in
+  assert (inv h 32);
+  assert (Seq.slice (B.as_seq h0 b1) 0 32 `Seq.equal` (B.as_seq h0 b1));
+  assert (Seq.slice (B.as_seq h0 b2) 0 32 `Seq.equal` (B.as_seq h0 b2));
+  B.gsub_zero_length b1;
+  assert (B.gsub b1 0ul 32ul == b1);
+  assert (as_hash_value b1 h ==
+          aggregate_hash_value (as_hash_value b1 h0) (as_hash_value b2 h0))
+
+let v_hash (s:state) (h:HS.mem)
+  : GTot hash_value_t
+  = as_hash_value (B.get h s 0).acc h
+
+#push-options "--fuel 1 --z3rlimit 20 --query_stats"
 let add s b l =
   let _ = allow_inversion state_s in
   let h0 = ST.get () in
+  let b = B.sub b 0ul (Ghost.hide l) in
   assert (invariant h0 s);
   push_frame ();
-  let { acc; seen; key } = !* s in
+  let s0 = !* s in
+  let { acc; seen; key } = s0 in
   let h1 = ST.get () in
   assert (invariant h1 s);
   let tmp = B.alloca 0uy 32ul in
@@ -97,8 +206,14 @@ let add s b l =
   assert_norm (64 < pow2 32);
   assert_norm (64 <= Hacl.Blake2b_32.max_key);
   Hacl.Blake2b_32.blake2b 32ul tmp l b 64ul key;
-  xor_inplace acc tmp;
+  let h2 = ST.get () in
+  assert (B.as_seq h2 tmp == hash_value (B.as_seq h1 b));
+  aggregate_hash_value_buf acc tmp;
   seen *= G.hide (B.as_seq h1 b :: B.deref h1 seen);
+  let h = ST.get () in
+  assert (v_hash s h ==
+                aggregate_hash_value (v_hash s h0)
+                                     (hash_value (B.as_seq h0 b)));
   pop_frame ()
 #pop-options
 
