steel/Veritas.Steel.PRFSetHash.fsti
@@ -13,6 +13,7 @@ module U64 = FStar.UInt64
 module T = Veritas.Formats.Types
 open Veritas.Steel.VerifierModel
 open Veritas.ThreadStateModel
+module AT = Steel.Effect.Atomic
 val prf_set_hash : Type0
 
 // AF: Internally, should probably be implemented with a ghost reference to the model_hash
@@ -57,6 +58,17 @@ val prf_update_hash (p:prf_set_hash) (r:T.record) (t:T.timestamp) (thread_id:T.t
     (requires fun _ -> True)
     (ensures fun h0 _ h1 -> v_hash p h1 == model_update_hash (v_hash p h0) r t thread_id)
 
+let prf_update_hash p r t thread_id =
+  let open Veritas.Formats.Types in
+  let srec = {
+    sr_record = r;
+    sr_timestamp = t;
+    sr_thread_id = thread_id;
+  } in
+  let a = Steel.Array.malloc 0uy 184ul in
+  let n = Veritas.Formats.serialize_stamped_record a srec in
+  sladmit()
+
 module A = Steel.Array
 module U8 = FStar.UInt8
 
@@ -70,3 +82,20 @@ val prf_read_hash (p:prf_set_hash) (out:A.array U64.t)
       A.length out == 4 /\
       v_hash p h0 == v_hash p h1 /\
       as_model_hash (A.asel out h1) == v_hash p h1)
+
+module MSH = Veritas.MultiSetHash
+val prf_hash_agg (a0 a1:A.array U64.t)
+  : Steel unit
+    (A.varray a0 `star` A.varray a1)
+    (fun _ -> A.varray a0 `star` A.varray a1)
+    (requires fun _ ->
+      A.length a0 == 4 /\
+      A.length a1 == 4)
+    (ensures fun h0 _ h1 ->
+      A.length a0 == 4 /\
+      A.length a1 == 4 /\
+      as_model_hash (A.asel a1 h0) ==
+         as_model_hash (A.asel a1 h1) /\
+      as_model_hash (A.asel a0 h1) ==
+        MSH.ms_hashfn_agg (as_model_hash (A.asel a0 h0))
+                          (as_model_hash (A.asel a1 h0)))
